code/mpfr/MPFR.Sub1sp1.fst
@@ -116,21 +116,6 @@ let mpfr_sub1sp1_any_post_cond h0 s h1 (a:mpfr_ptr) b c (p:mpfr_reg_prec_t) rnd_
         (rb_def r (I64.v p) = (v s.rb <> 0)) /\
         (sb_def r (I64.v p) = (v s.sb <> 0)) /\
         (high_mant r (I64.v p)).sign = (as_normal h1 a).sign)
-        
-inline_for_extraction val mpfr_sub1sp1_eq:
-    a:mpfr_ptr -> b:mpfr_ptr -> c:mpfr_ptr ->
-    ap:buffer mp_limb_t -> bp:buffer mp_limb_t -> cp:buffer mp_limb_t ->
-    bx:mpfr_reg_exp_t ->cx:mpfr_reg_exp_t
-    ->rnd_mode:mpfr_rnd_t->
-    p:mpfr_reg_prec_t -> sh:mpfr_reg_prec_t -> Stack state
-    (requires (fun h-> mpfr_sub1sp1_pre_cond h a b c p /\
-    mpfr_sub1sp1_pre_cond_2 h a b c bx cx ap bp cp p sh /\
-    I64.(bx=^cx) /\
-    I64.(as_val h bp<>as_val h cp)
-    ))
-    (ensures (fun h0 s h1->
-    let exact=sub1sp_exact (as_fp h0 b) (as_fp h0 c) in
-    mpfr_sub1sp1_any_post_cond h0 s h1 a b c p rnd_mode exact))
 
 val mpfr_sub1sp1_eq_rb_sb_lemma:
     b:mpfr_reg_fp -> c:mpfr_reg_fp -> p:pos -> Lemma
@@ -210,22 +195,41 @@ let mpfr_sub1sp1_eq_value_lemma a b c cnt p=
     lemma_fp_eq_cross a k
     
 
+inline_for_extraction val mpfr_sub1sp1_eq:
+    a:mpfr_ptr -> b:mpfr_ptr -> c:mpfr_ptr ->
+    ap:buffer mp_limb_t -> bp:buffer mp_limb_t -> cp:buffer mp_limb_t ->
+    bx:mpfr_reg_exp_t ->cx:mpfr_reg_exp_t
+    ->rnd_mode:mpfr_rnd_t->
+    p:mpfr_reg_prec_t -> sh:mpfr_reg_prec_t -> Stack state
+    (requires (fun h-> mpfr_sub1sp1_pre_cond h a b c p /\
+    mpfr_sub1sp1_pre_cond_2 h a b c bx cx ap bp cp p sh /\
+    I64.(bx=^cx) /\
+    I64.(as_val h bp<>as_val h cp)
+    ))
+    (ensures (fun h0 s h1->
+    let exact=sub1sp_exact (as_fp h0 b) (as_fp h0 c) in
+    mpfr_sub1sp1_any_post_cond h0 s h1 a b c p rnd_mode exact))
+
 let mpfr_sub1sp1_eq a b c ap bp cp bx cx rnd_mode p sh =
     let h0=ST.get() in
     let vb= v bp.(0ul) in
     let vc= v cp.(0ul) in
     let vsh= I64.(v sh) in 
-    if(cp.(0ul)>^bp.(0ul)) then begin admit();
+    if(cp.(0ul)>^bp.(0ul)) then begin 
       let a0=cp.(0ul) -^ bp.(0ul) in
       let cnt=count_leading_zeros a0 in
-     // mpfr_SET_OPPOSITE_SIGN a b;
+      mpfr_SET_SIGN a (mpfr_NEG_SIGN (mpfr_SIGN b));(*mpfr_SET_OPPOSITE_SIGN does exactly this, but makes it harder to check*)
       ap.(0ul) <- a0<<^cnt;
       lemma_mod_distr_sub_zero vc vb (pow2 vsh);
       lemma_shift_left_mod_pow2 a0 cnt vsh;
-      let h1=ST.get() in
       let bx=I64.(bx -^ (uint32_to_int64 cnt)) in
-      mk_state sh bx  0uL 0uL
-    end else begin 
+      let h1=ST.get() in
+      shift_left_value_lemma (v a0) (U32.v cnt);
+      lemma_small_mod (v a0*pow2 (U32.v cnt)) (pow2 64);
+      mpfr_sub1sp1_eq_value_lemma ({(as_normal h1 a) with exp=I64.v bx}) (as_reg_fp h0 b) (as_reg_fp h0 c) (U32.v cnt) (I64.v p);
+      mpfr_sub1sp1_eq_rb_sb_lemma (as_reg_fp h0 b) (as_reg_fp h0 c) (I64.v p);
+      mk_state sh bx 0uL 0uL
+    end else begin
       let a0=bp.(0ul) -^ cp.(0ul) in
       let cnt=count_leading_zeros a0 in
       mpfr_SET_SAME_SIGN a b;
@@ -238,8 +242,198 @@ let mpfr_sub1sp1_eq a b c ap bp cp bx cx rnd_mode p sh =
       lemma_small_mod (v a0*pow2 (U32.v cnt)) (pow2 64);
       mpfr_sub1sp1_eq_value_lemma ({(as_normal h1 a) with exp=I64.v bx}) (as_reg_fp h0 b) (as_reg_fp h0 c) (U32.v cnt) (I64.v p);
       mpfr_sub1sp1_eq_rb_sb_lemma (as_reg_fp h0 b) (as_reg_fp h0 c) (I64.v p);
-      let t=mk_state sh bx 0uL 0uL in t
+      mk_state sh bx 0uL 0uL
     end
+
+val lemma_gt_exp_sub1sp:  b:mpfr_reg_fp -> c:mpfr_reg_fp -> Lemma
+ (requires (b.exp>c.exp))
+ (ensures (gt (eval_abs b) (eval_abs c)))
+
+let lemma_gt_exp_sub1sp b c=
+    let eb,ec=(eval_abs b),(eval_abs c) in
+    let elb=min eb.exponent ec.exponent in
+    assert(b.limb>=pow2 (b.len-1));
+    assert(b.limb*(pow2 (b.exp-b.len-elb))>=pow2 (b.len-1)*(pow2 (b.exp-b.len-elb)));
+    lemma_pow2_mul (b.len-1) (b.exp-b.len-elb);
+    assert(b.limb*(pow2 (b.exp-b.len-elb))>=pow2 (b.exp-1-elb));
+    assert(pow2 c.len>c.limb);
+    lemma_pow2_le (c.exp-elb) (b.exp-1-elb);
+    assert(pow2 (b.exp-1-elb)>=pow2 (c.exp-elb));
+    lemma_pow2_mul c.len (c.exp-c.len-elb);
+    assert(b.limb*(pow2 (b.exp-b.len-elb))>=(pow2 c.len)*(pow2 (c.exp-c.len-elb)))
+
+val lemma_sub1sp1_gt_exp_2_limb1: b:mpfr_reg_fp -> c:mpfr_reg_fp -> p:pos{b.prec=p /\ c.prec=p /\ p<64} -> Lemma
+    (requires (b.exp>c.exp /\ b.exp-c.exp>=64 /\ b.limb<>v mpfr_LIMB_HIGHBIT))
+    (ensures (let r=sub1sp_exact b c in
+        let d=b.exp-c.exp in
+        r.limb>=pow2 (63+d)
+    ))
+
+let lemma_sub1sp1_gt_exp_2_limb1 b c p=
+    lemma_gt_exp_sub1sp b c;
+    let d=b.exp-c.exp in
+    let r=sub1sp_exact b c in
+    assert(r.limb=b.limb*pow2 d-c.limb);
+    assert(c.limb<pow2 c.len);
+    assert(c.len<=d);
+    lemma_pow2_le c.len d;
+    assert(r.limb>=(b.limb-1)*pow2 d);
+    assert(b.limb-1>=pow2 63);
+    lemma_pow2_mul 63 d;
+    assert(r.limb>=pow2 (63+d))
+
+val lemma_sub1sp1_gt_exp_2_limb2: b:mpfr_reg_fp -> c:mpfr_reg_fp -> p:pos{b.prec=p /\ c.prec=p /\ p<64} -> Lemma
+    (requires (b.exp>c.exp /\ b.exp-c.exp>=64 /\ b.limb<>v mpfr_LIMB_HIGHBIT))
+    (ensures (let r=sub1sp_exact b c in
+        let d=b.exp-c.exp in
+        r.limb<pow2 (64+d)
+    ))
+
+let lemma_sub1sp1_gt_exp_2_limb2 b c p=
+    lemma_gt_exp_sub1sp b c;
+    let d=b.exp-c.exp in
+    let r=sub1sp_exact b c in
+    assert(r.limb=b.limb*pow2 d-c.limb);
+    assert(r.limb<=b.limb*pow2 d);
+    assert(b.limb<pow2 b.len);
+    assert(b.len=64);
+    lemma_pow2_mul 64 d;
+    assert(r.limb<pow2 (64+d))
+
+val lemma_sub1sp1_gt_rb_sb_exp_2:  b:mpfr_reg_fp -> c:mpfr_reg_fp -> p:pos{b.prec=p /\ c.prec=p /\ p<64} -> Lemma
+    (requires (b.exp>c.exp /\ b.exp-c.exp>=64 /\ b.limb<>v mpfr_LIMB_HIGHBIT))
+    (ensures (let r=sub1sp_exact b c in
+        r.exp=b.exp /\ rb_def r p /\ sb_def r p
+    ))
+
+let lemma_sub1sp1_gt_rb_sb_exp_2 b c p=
+    lemma_gt_exp_sub1sp b c;
+    let d=b.exp-c.exp in
+    let r=sub1sp_exact b c in
+    lemma_sub1sp1_gt_exp_2_limb1 b c p;
+    lemma_sub1sp1_gt_exp_2_limb2 b c p;
+    lemma_pow2_nbits_rev r.limb (64+d);
+    (*sb*)
+    lemma_pow2_le 64 (r.len-p-1);
+    lemma_small_mod c.limb (pow2 (r.len - p - 1));
+    let cm=c.limb % pow2 (r.len - p - 1) in
+    lemma_pow2_mod_mod_zero b.limb (64-p) (r.len-p-d);
+    lemma_mod_mul b.limb (pow2 (r.len-p-d)) (pow2 d);
+    lemma_pow2_mul (r.len-p-d) d;
+    lemma_pow2_mod_mod_zero (b.limb*pow2 d) (r.len-p) (r.len-p-1);
+    lemma_mod_distr_sub (b.limb * pow2 d) c.limb (pow2 (r.len - p - 1));
+    (*rb*)
+    lemma_pow2_le 64 (r.len-p);
+    lemma_small_mod c.limb (pow2 (r.len - p));
+    lemma_mod_distr_sub (b.limb * pow2 d) c.limb (pow2 (r.len - p));
+    lemma_small_mod_neg cm (pow2 (r.len - p));
+    lemma_small_mod_neg cm (pow2 (r.len - p-1));
+    rb_value_lemma r p
+
+val lemma_sub1sp1_gt_value_2:  b:mpfr_reg_fp -> c:mpfr_reg_fp -> p:pos{b.prec=p /\ c.prec=p /\ p<64} -> Lemma
+    (requires (b.exp>c.exp /\ b.exp-c.exp>=64 /\ b.limb<>v mpfr_LIMB_HIGHBIT))
+    (ensures (let r=sub1sp_exact b c in
+       (b.limb-(pow2 (64-p))) * pow2 (high_mant r p).len = (high_mant r p).limb * (pow2 64)
+    ))
+
+let lemma_sub1sp1_gt_value_2 b c p=
+    lemma_gt_exp_sub1sp b c;
+    let d=b.exp-c.exp in
+    let r=sub1sp_exact b c in
+    lemma_sub1sp1_gt_exp_2_limb1 b c p;
+    lemma_sub1sp1_gt_exp_2_limb2 b c p;
+    lemma_pow2_nbits_rev r.limb (64+d);
+    lemma_pow2_mod_mod_zero b.limb (64-p) (r.len-p-d);
+    lemma_mod_mul b.limb (pow2 (r.len-p-d)) (pow2 d);
+    lemma_pow2_mul (r.len-p-d) d;
+    lemma_pow2_le 64 (r.len-p);
+
+    lemma_pow2_mul (r.len-64) (64-p);
+    lemma_div_div (b.limb*pow2 d) (pow2 d) (pow2 (64-p));
+    lemma_multiple_div b.limb (pow2 d);
+    //!  assert((b.limb*pow2 d)/(pow2 (r.len-p))=b.limb/(pow2 (64-p)));
+    lemma_small_div_neg c.limb (pow2 (r.len - p));
+    lemma_div_distr (b.limb*pow2 d) (0-c.limb) (pow2 (r.len-p));
+    //! assert((high_mant r p).limb*(pow2 64)=(b.limb / pow2 (64 - p) - 1)*(pow2 (r.len-p))*(pow2 64));
+    lemma_paren_mul_right (b.limb / pow2 (64 - p) - 1) (pow2 (r.len-p)) (pow2 64);
+    lemma_pow2_mul (r.len-p) 64;
+    lemma_paren_mul_right (b.limb / pow2 (64 - p) - 1) (pow2 (64-p)) (pow2 r.len);
+    lemma_pow2_mul r.len (64-p);
+    //! assert((high_mant r p).limb*(pow2 64)=((b.limb / pow2 (64 - p) - 1)*(pow2 (64-p)))*pow2 r.len);
+    lemma_distr_sub_left (b.limb/pow2 (64-p)) 1 (pow2 (64-p));
+    lemma_div_mul b.limb (pow2 (64-p))
+  
+
+val lemma_sub1sp1_gt_rb_sb_exp_3:  b:mpfr_reg_fp -> c:mpfr_reg_fp -> p:pos{b.prec=p /\ c.prec=p /\ p<64} -> Lemma
+    (requires (b.exp>c.exp /\ b.exp-c.exp>=64 /\ b.limb=v mpfr_LIMB_HIGHBIT))
+    (ensures (let r=sub1sp_exact b c in
+        r.exp=b.exp-1 /\ 
+        rb_def r p=(p<63||b.exp-c.exp>64||c.limb=v mpfr_LIMB_HIGHBIT) /\
+        sb_def r p=(p<63||b.exp-c.exp>64||c.limb<>v mpfr_LIMB_HIGHBIT)
+    ))
+
+let lemma_sub1sp1_gt_rb_sb_exp_3 b c p=
+    lemma_gt_exp_sub1sp b c;
+    let d=b.exp-c.exp in
+    let r=sub1sp_exact b c in
+    lemma_pow2_mul 63 d;
+    lemma_pow2_le 64 (62+d);
+    lemma_pow2_nbits_rev r.limb (63+d);
+    
+    lemma_mod_product_zero b.limb (pow2 d) (pow2 (64-p)) (pow2 d);
+    lemma_pow2_mul (64-p) d;
+    
+    lemma_pow2_mod_mod_zero (b.limb*pow2 d) (64-p+d) (62+d-p);
+    lemma_small_mod 0 (pow2 (62+d-p));
+    lemma_mod_distr_sub (b.limb*pow2 d) c.limb (pow2 (62+d-p));
+    lemma_mod_distr_sub 0 c.limb (pow2 (62+d-p));
+
+    lemma_pow2_mod_mod_zero (b.limb*pow2 d) (64-p+d) (63+d-p);
+    lemma_small_mod 0 (pow2 (63+d-p));
+    lemma_mod_distr_sub (b.limb*pow2 d) c.limb (pow2 (63+d-p));
+    lemma_mod_distr_sub 0 c.limb (pow2 (63+d-p));
+
+    rb_value_lemma r p;
+    if p<63||d>64 then begin
+      lemma_pow2_le 64 (62+d-p);
+      lemma_small_mod_neg c.limb (pow2 (62+d-p));
+      lemma_pow2_le 64 (63+d-p);
+      lemma_small_mod_neg c.limb (pow2 (63+d-p))
+    end
+
+    
+
+val lemma_sub1sp1_gt_value_3:  b:mpfr_reg_fp -> c:mpfr_reg_fp -> p:pos{b.prec=p /\ c.prec=p /\ p<64} -> Lemma
+    (requires (b.exp>c.exp /\ b.exp-c.exp>=64 /\ b.limb=v mpfr_LIMB_HIGHBIT))
+    (ensures (let r=sub1sp_exact b c in
+       (pow2 64-pow2 (64-p)) * pow2 (high_mant r p).len = (high_mant r p).limb * (pow2 64)
+    ))
+
+let lemma_sub1sp1_gt_value_3 b c p=
+    lemma_gt_exp_sub1sp b c;
+    let d=b.exp-c.exp in
+    let r=sub1sp_exact b c in
+    lemma_pow2_mul 63 d;
+    lemma_pow2_le 64 (62+d);
+    lemma_pow2_nbits_rev r.limb (63+d);
+    
+    lemma_mod_product_zero b.limb (pow2 d) (pow2 (64-p)) (pow2 d);
+    lemma_pow2_mul (64-p) d;
+
+    lemma_pow2_mod_mod_zero (b.limb*pow2 d) (64-p+d) (63+d-p);
+    lemma_small_mod 0 (pow2 (63+d-p));
+    
+    lemma_div_distr (b.limb*pow2 d) (0-c.limb) (pow2 (63+d-p));
+    lemma_pow2_mul (63+d-p) p;
+    lemma_multiple_div (pow2 p) (pow2 (63+d-p));
+    lemma_pow2_le 64 (63+d-p);
+    lemma_small_div_neg c.limb (pow2 (63+d-p));
+    lemma_distr_sub_left (pow2 p) 1 (pow2 (63+d-p));
+    lemma_distr_sub_left (pow2 (63+d)) (pow2 (63+d-p)) (pow2 64);
+    lemma_distr_sub_left (pow2 (64)) (pow2 (64-p)) (pow2 (63+d));
+    lemma_pow2_mul (63+d-p) 64;
+    lemma_pow2_mul (64-p) (63+d)
+    
 
 inline_for_extraction val mpfr_sub1sp1_gt:
     a:mpfr_ptr -> b:mpfr_ptr -> c:mpfr_ptr ->
@@ -250,25 +444,77 @@ inline_for_extraction val mpfr_sub1sp1_gt:
     (requires (fun h->
     mpfr_sub1sp1_pre_cond h a b c p /\
     mpfr_sub1sp1_pre_cond_2 h a b c bx cx ap bp cp p sh /\
-    I64.(bx >^ cx)))
-    (ensures (fun h0 t h1->
-    let exact=sub1sp_exact (as_fp h0 b) (as_fp h0 c) in
-    mpfr_sub1sp1_any_post_cond h0 t h1 a b c p rnd_mode exact))
+    I64.(bx>^cx)))
+    (ensures (fun h0 s h1->
+   (* let exact=sub1sp_exact (as_fp h0 b) (as_fp h0 c) in*)
+    (*mpfr_sub1sp1_any_post_cond h0 s h1 a b c p rnd_mode exact*)  (* Memory safety *)
+        mpfr_live h1 a /\ mpfr_live h1 b /\ mpfr_live h1 c /\
+        length (as_struct h1 a).mpfr_d = 1 /\
+        length (as_struct h1 b).mpfr_d = 1 /\ length (as_struct h1 c).mpfr_d = 1 /\
+        modifies_2 a (as_struct h1 a).mpfr_d h0 h1 /\ normal_cond h1 a /\ 
+        (as_normal h1 a).prec=I64.v p /\ (as_struct h0 a).mpfr_d==(as_struct h1 a).mpfr_d /\
+        (*Functional correctness*)
+        I64.(v ((as_struct h0 a).mpfr_prec)=v p) /\
+        I64.(v ((as_struct h0 b).mpfr_prec)=v p) /\
+        I64.(v ((as_struct h0 c).mpfr_prec)=v p) /\
+        mpfr_reg_cond h0 b /\ mpfr_reg_cond h0 c /\
+        (let r = sub1sp_exact (as_reg_fp h0 b) (as_reg_fp h0 c) in
+        normal_fp_cond r /\
+        I64.(s.bx<=^mpfr_EMAX) /\
+        as_val h1 (as_struct h1 a).mpfr_d * pow2 (high_mant r (I64.v p)).len = (high_mant r (I64.v p)).limb * (pow2 64) /\
+        I64.v s.sh = I64.v gmp_NUMB_BITS - I64.v p /\
+        I64.v s.bx =(high_mant r (I64.v p)).exp /\
+        (rb_def r (I64.v p) = (v s.rb <> 0)) /\
+        (sb_def r (I64.v p) = (v s.sb <> 0)) /\
+        (high_mant r (I64.v p)).sign = (as_normal h1 a).sign)))
 
-let mpfr_sub1sp1_gt a b c ap bp cp bx cx rnd_mode p sh =admit()(*;
-    let d = I64.(bx-^cx) in
-    let mask = mpfr_LIMB_MASK (int64_to_uint32 sh) in
-    if I64.(d <^ gmp_NUMB_BITS) then begin
-      let sb=0uL -^ (cp.(0ul) <<^ (int64_to_uint32 I64.(gmp_NUMB_BITS -^ d))) in
-      let a0_tmp = bp.(0ul) -^ (if v sb=0 then 0uL else 1uL) -^ (cp.(0ul)>>^(int64_to_uint32 d)) in
-      assert(v a0_tmp>0);
-      let cnt=count_leading_zeros a0_tmp in
-      let a0=if U32.(v cnt)>0 then (a0_tmp<<^cnt) |^ (sb>>^U32.(int64_to_uint32 gmp_NUMB_BITS -^ cnt)) else a0_tmp in
-      ap.(0ul)<-a0 &^ (lognot mask);
-      mpfr_sub1sp1_round a ap sh bx 0uL 0uL rnd_mode
+let mpfr_sub1sp1_gt a b c ap bp cp bx cx rnd_mode p sh =
+    let h0=ST.get() in
+    mpfr_SET_SAME_SIGN a b;
+    let d=I64.(bx-^cx) in
+    let bp0ul=bp.(0ul) in
+    let cp0ul=cp.(0ul) in
+    let mask=mpfr_LIMB_MASK (int64_to_uint32 sh) in
+    lemma_gt_exp_sub1sp (as_reg_fp h0 b) (as_reg_fp h0 c);
+    if(I64.(d<^64L)) then begin 
+      let sb=0uL-^(cp0ul<<^(int64_to_uint32 I64.(gmp_NUMB_BITS-^d))) in
+      let a0=bp0ul -^ (if sb=0 then 0uL else 1uL) -^ (cp0ul >>^ (int64_to_uint32 d)) in
+      let cnt=count_leading_zeros a0 in
+      //let a0=0 in
+      let rb=a0 &^ (mpfr_LIMB_ONE <<^ (int64_to_uint32 I64.(sh-^1L))) in
+      let t=mk_state sh I64.(bx-^(uint32_to_int64 cnt)) rb sb in t
+    end else begin admit();
+      if(bp0ul>^mpfr_LIMB_HIGHBIT) then begin
+        assert((v bp0ul)%(pow2 (I64.v sh))=0);
+        lemma_mod_ge_zero (v bp0ul) (pow2 (I64.v sh));
+        lemma_pow2_mod 63 (I64.v sh);
+        lemma_mod_distr_sub_zero (v bp0ul) (v mpfr_LIMB_HIGHBIT) (pow2 (I64.v sh));
+        lemma_mod_ge_zero (v bp0ul-v mpfr_LIMB_HIGHBIT) (pow2 (I64.v sh));
+        assert(bp0ul -^ mpfr_LIMB_HIGHBIT >=^ (mpfr_LIMB_ONE <<^ (int64_to_uint32 sh)));
+        assert((bp0ul -^ (mpfr_LIMB_ONE <<^ (int64_to_uint32 sh)))>=^mpfr_LIMB_HIGHBIT);
+        ap.(0ul) <- bp0ul -^ (mpfr_LIMB_ONE <<^ (int64_to_uint32 sh));
+        let h1=ST.get() in
+        shift_left_value_lemma (v mpfr_LIMB_ONE) (I64.v sh);
+        lemma_pow2_mul_mod (v mpfr_LIMB_ONE) (I64.v sh) 64;
+        lemma_multiple_mod (v mpfr_LIMB_ONE%pow2 (64-(I64.v sh))) (pow2 (I64.v sh));
+        lemma_mod_distr_sub_zero (v bp0ul) (v (mpfr_LIMB_ONE <<^ (int64_to_uint32 sh))) (pow2 (I64.v sh));
+        lemma_sub1sp1_gt_rb_sb_exp_2 (as_reg_fp h0 b) (as_reg_fp h0 c) (I64.v p);
+        lemma_sub1sp1_gt_value_2 (as_reg_fp h0 b) (as_reg_fp h0 c) (I64.v p);
+        mk_state sh bx 1uL 1uL
+      end else begin
+        let rb=(I64.(sh>^1L||d>^gmp_NUMB_BITS)||cp0ul=mpfr_LIMB_HIGHBIT) in
+        let sb=(I64.(sh>^1L||d>^gmp_NUMB_BITS)||cp0ul<>mpfr_LIMB_HIGHBIT) in
+        ap.(0ul) <- (UInt64.lognot mask);
+        let h1=ST.get() in
+        lemma_lognot_value mask;
+        lemma_pow2_mod 64 (I64.v sh);
+        lemma_mod_distr_sub_zero (pow2 64) (pow2 (I64.v sh)) (pow2 (I64.v sh));
+        lemma_sub1sp1_gt_rb_sb_exp_3 (as_reg_fp h0 b) (as_reg_fp h0 c) (I64.v p);
+        lemma_sub1sp1_gt_value_3 (as_reg_fp h0 b) (as_reg_fp h0 c) (I64.v p);
+        assert(I64.(v (bx-^1L))=(sub1sp_exact (as_reg_fp h0 b) (as_reg_fp h0 c)).exp);
+        mk_state sh I64.(bx-^1L) (if rb then 1uL else 0uL) (if sb then 1uL else 0uL)
+      end
     end
-    else mpfr_RET 0l
-*)
 
 (* specifications for mpfr_sub1sp1 *)
 val mpfr_sub1sp1: a:mpfr_ptr -> b:mpfr_ptr -> c:mpfr_ptr ->
@@ -277,6 +523,78 @@ val mpfr_sub1sp1: a:mpfr_ptr -> b:mpfr_ptr -> c:mpfr_ptr ->
     (ensures  (fun h0 t h1 ->
     let exact=sub1sp_exact (as_fp h0 b) (as_fp h0 c) in
     mpfr_sub1sp1_post_cond h0 t h1 a b c p rnd_mode exact))
+
+val lemma_underflow_fp_value: f:normal_fp -> p:nat{mpfr_PREC_COND p} -> Lemma
+    (requires (f.exp<mpfr_EMIN_spec))
+    (ensures (eval_abs f<.mpfr_underflow_bound p))
+
+let lemma_underflow_fp_value f p=
+    let d1=eval_abs f in
+    let d2=mpfr_underflow_bound p in
+    let elb=min d1.exponent d2.exponent in
+    assert(f.limb<pow2 f.len);
+    assert(f.limb*pow2(f.exp-f.len-elb)<pow2 f.len*pow2 (f.exp-f.len-elb));
+    lemma_pow2_mul f.len (f.exp-f.len-elb);
+    assert(f.limb*pow2(f.exp-f.len-elb)<pow2 (f.exp-elb));
+    lemma_pow2_le (f.exp-elb) (mpfr_EMIN_spec-1-elb);
+    assert(pow2 (f.exp-elb)<=pow2 (mpfr_EMIN_spec-1-elb));
+    let l=prec_to_len p in
+    lemma_pow2_mul (l-1) (mpfr_EMIN_spec-l-elb);
+    assert(pow2 (mpfr_EMIN_spec-1-elb)<=d2.significand*pow2 (d2.exponent-elb))
+
+let my_cond f p=(*f.exp-f.prec>=mpfr_EMIN_spec-p*)(*(f.exp-mpfr_EMIN_spec+p>=0) /\ (f.limb*pow2 (f.exp-mpfr_EMIN_spec+p))%(pow2 f.len)=0*)mpfr_EMIN_spec+f.len-f.exp-p<0 \/ f.limb%pow2 (mpfr_EMIN_spec+f.len-f.exp-p)=0
+
+val lemma_mc_1: f:mpfr_fp -> p:pos{p=f.prec} -> Lemma
+    (requires (MPFR_NUM? f.flag))
+    (ensures (my_cond f p))
+  
+let lemma_mc_1 f p=assert(f.exp>=mpfr_EMIN_spec);
+    assert(f.limb%pow2(f.len-p)=0);
+    if(mpfr_EMIN_spec+f.len-f.exp-p>=0)then begin
+      lemma_pow2_mod_mod_zero f.limb (f.len-p) (mpfr_EMIN_spec+f.len-f.exp-p)
+    end
+   (* assert(f.limb%pow2 (f.len-p)=0);
+    lemma_mod_product_zero f.limb (pow2 p) (pow2 (f.len-p)) (pow2 p);
+    lemma_pow2_mul (f.len-p) p;
+    assert((f.limb*pow2 p)%(pow2 f.len)=0);
+    lemma_pow2_mul (f.exp-mpfr_EMIN_spec) p;
+    lemma_mul_mod_zero (f.limb*pow2 p) (pow2 (f.exp-mpfr_EMIN_spec)) (pow2 f.len)*)
+
+val lemma_mc_2: b:mpfr_reg_fp -> c:mpfr_reg_fp{b.prec=c.prec} -> p:pos -> Lemma
+    (requires (my_cond b p /\ my_cond c p))
+    (ensures (my_cond (sub1sp_exact b c) p))
+
+let lemma_mc_2 b c p=let exact=sub1sp_exact b c in
+(* fabs (eval_abs a -. eval_abs b) =. eval_abs r*)
+(*assert(eval_abs a)
+assume(exact.flag=MPFR_NUM)*)admit()
+
+val lemma_underflow_round: f:normal_fp -> p:mpfr_prec_t -> rnd_mode:mpfr_rnd_t -> Lemma
+    (requires (my_cond f (I64.v p) /\ f.exp<mpfr_EMIN_spec))
+    (ensures (let rnd=(round_def f (I64.v p) rnd_mode) in
+    eval_abs f=.eval_abs rnd))
+
+let lemma_underflow_round f p rnd_mode=();admit()
+
+(*
+let test_cond x rnd_mode sign h0 t h1=let p = (as_struct h1 x).mpfr_prec in
+        mpfr_live h1 x /\ mpfr_modifies x h0 h1 /\
+        mpfr_valid_cond h1 x /\ (as_struct h1 x).mpfr_sign = sign /\
+	(forall (exact:normal_fp{exact.sign = I32.v sign /\ exact.exp < mpfr_EMIN_spec}).
+	as_fp h1 x == mpfr_underflow_spec exact (I64.v p) rnd_mode /\
+	I32.v t = mpfr_underflow_ternary_spec exact (I64.v p) rnd_mode)
+        
+val my_lemma   (requires ((r == mpfr_underflow_spec a p rnd_mode /\
+               t = mpfr_underflow_ternary_spec a p rnd_mode) /\
+	       eval_abs (round_def a p rnd_mode) <. mpfr_underflow_bound p /\
+	       (MPFR_RNDN? rnd_mode ==>
+	        eval_abs (rndn_def a p) >. fdiv_pow2 (mpfr_underflow_bound p) 1)))*)
+
+val my_lemma: a:I64.t -> b:I64.t -> Lemma
+  (requires I64.(a <^ b /\ not (a<^ (b -^ 1L))))
+  (ensures I64.(a =^ (b -^ 1L)))
+
+let my_lemma a b=admit()
 
 let mpfr_sub1sp1 a b c rnd_mode p =
     let bx=mpfr_GET_EXP b in
@@ -294,34 +612,56 @@ let mpfr_sub1sp1 a b c rnd_mode p =
     let st=if I64.(bx =^ cx) then begin
       mpfr_sub1sp1_eq a b c ap bp cp bx cx rnd_mode p sh
     end else begin  admit();
-   let b,c,bx,cx,bp,cp=(if I64.(bx >=^ cx) then (mpfr_SET_SAME_SIGN a b;b,c,bx,cx,bp,cp) else (mpfr_SET_OPPOSITE_SIGN a b;c,b,cx,bx,cp,bp)) in       
+    let b,c,bx,cx,bp,cp=(if I64.(bx >=^ cx) then (mpfr_SET_SAME_SIGN a b;b,c,bx,cx,bp,cp) else (mpfr_SET_OPPOSITE_SIGN a b;c,b,cx,bx,cp,bp)) in       
     mpfr_sub1sp1_gt a b c ap bp cp bx cx rnd_mode p sh
     end in 
     let h1 = ST.get() in
     if I64.(st.bx <^ mpfr_EMIN) then begin 
         let s = mpfr_SIGN a in
         let ap0ul=ap.(0ul) in
-        let t = if(rnd_mode=MPFR_RNDN(*&&(I64.(st.bx<^(mpfr_EMIN-^1L))||ap0ul=mpfr_LIMB_HIGHBIT)*)) then begin
-            ignore(mpfr_underflow a MPFR_RNDZ s);admit()
-        end else begin
+        let t = if(rnd_mode=MPFR_RNDN&&(I64.(st.bx<^(mpfr_EMIN-^1L))||ap0ul=mpfr_LIMB_HIGHBIT)) then begin
+            let t=mpfr_underflow a MPFR_RNDZ s in
+            admit()//(eval_abs low <. ulp_p high (p + 1))
+        end else begin admit();
             let t=mpfr_underflow a rnd_mode s in
             let h2=ST.get() in
-            
-            assume(I64.v p<=(sub1sp_exact (as_reg_fp h0 b) (as_reg_fp h0 c)).prec);
+(*
+           (* lemma_mc_1 (as_reg_fp h0 b) (I64.v p);
+            lemma_mc_1 (as_reg_fp h0 c) (I64.v p);
+            assert(my_cond (as_reg_fp h0 b) (I64.v p));
+            assert(my_cond (as_reg_fp h0 c) (I64.v p));*)
             (let exact=(sub1sp_exact (as_reg_fp h0 b) (as_reg_fp h0 c)) in
             let p=(as_struct h2 a).mpfr_prec in
-            assert((as_fp h2 a)==mpfr_underflow_spec exact (I64.v p) rnd_mode);
-            assert(I32.v t=mpfr_underflow_ternary_spec exact (I64.v p) rnd_mode);
-           // assert(mpfr_PREC_COND (I64.v p));
-           assume((round_def exact (I64.v p) rnd_mode).exp < mpfr_EMIN_spec);admit();
-            assert(eval_abs (round_def exact (I64.v p) rnd_mode) <. mpfr_underflow_bound (I64.v p) );admit();
-            assert( (MPFR_RNDN? rnd_mode ==>
+ 
+//assert(my_cond exact (I64.v p));
+            assert(exact.exp<mpfr_EMIN_spec);
+            lemma_underflow_fp_value exact (I64.v p);
+            assert(eval_abs exact<.mpfr_underflow_bound (I64.v p));
+            assume(my_cond exact (I64.v p));
+            lemma_underflow_round exact p rnd_mode;
+            assert(eval_abs exact =. eval_abs (round_def exact (I64.v p) rnd_mode));
+            assert(eval_abs (round_def exact (I64.v p) rnd_mode) <. mpfr_underflow_bound (I64.v p));
+           // assume(not (MPFR_RNDN? rnd_mode));
+//assert(exact.exp=I64.v st.bx /\ exact.limb=v ap0ul);admit();
+          //  assert(exact.exp=mpfr_EMAX_spec-1(* /\ exact.limb<>v mpfr_LIMB_HIGHBIT*));admit();
+            if(MPFR_RNDN? rnd_mode) then begin
+            assert(not (I64.(st.bx<^(mpfr_EMIN-^1L))||ap0ul=mpfr_LIMB_HIGHBIT));
+            my_lemma st.bx mpfr_EMIN;
+            assert(I64.(st.bx=^(mpfr_EMIN-^1L)) && ap0ul <> mpfr_LIMB_HIGHBIT);
+          //  (eval_abs low <. ulp_p high (p + 1))
+            //assume(rndn_def exact (I64.v p)=add_one_ulp (rndz_def exact (I64.v p)));
+             assert(eval_abs (rndz_def exact (I64.v p)) >=. fdiv_pow2 (mpfr_underflow_bound (I64.v p)) 1);
+                assume(eval_abs (rndn_def exact (I64.v p)) >. fdiv_pow2 (mpfr_underflow_bound (I64.v p)) 1)
+            end;
+            assert((MPFR_RNDN? rnd_mode ==>
 	            eval_abs (rndn_def exact (I64.v p)) >. fdiv_pow2 (mpfr_underflow_bound (I64.v p)) 1)));
             assert(I64.v p=I64.v (as_struct h2 a).mpfr_prec);
 
             mpfr_underflow_post_cond_lemma (sub1sp_exact (as_reg_fp h0 b) (as_reg_fp h0 c)) (I64.v p) rnd_mode (I32.v t) (as_fp h2 a);
-            t
+*)            admit();t
         end in
+        
+
 	t
     end else begin admit();
         let t = mpfr_add1sp1_round a ap rnd_mode st in
@@ -331,3 +671,4 @@ let mpfr_sub1sp1 a b c rnd_mode p =
 	t
     end
  end
+ 
